translation

target_calculus.v
@@ -5,6 +5,7 @@ Require Import semilattice.
 Section TargetCalculus.
 
 Parameter label : Set.
+Parameter label_eq : forall (l1 l2 : label), {l1 = l2} + {~l1 = l2}.
 Parameter precedes : label -> label -> Prop.
 Parameter bottom : label.
 Parameter join : label -> label -> label.
@@ -78,8 +79,16 @@ Notation "s → t" := (full_step s t) (at level 70).
 
 Inductive star : term -> term -> Prop :=
 | StarR p : star p p
-| StarC x y z : x →@ y -> star y z -> star x z.
+| StarC x y z : x → y -> star y z -> star x z.
 Notation "s →* t" := (star s t) (at level 70).
+
+Lemma star_step s t :
+  s → t -> s →* t.
+Proof.
+  intros. eapply StarC.
+  + apply H.
+  + apply StarR.
+Qed.
 
 Lemma star_trans s t u :
   s →* t -> t →* u -> s →* u.
@@ -87,6 +96,72 @@ Proof.
   intros. revert u H0. induction H ; intros ; simpl.
   - assumption.
   - eapply StarC. eassumption. apply IHstar. assumption.
+Qed.
+
+Lemma pair_star_l s s' t:
+  s →* s' -> Pair s t →* Pair s' t.
+Proof.
+  intros ; induction H ; eauto using step, full_step, star.
+Qed.
+
+Lemma pair_star_r s t t' :
+  t →* t' -> Pair s t →* Pair s t'.
+Proof.
+  intros ; induction H ; eauto using step, full_step, star.
+Qed.
+
+Lemma pair_star s s' t t' :
+  s →* s' -> t →* t' ->  Pair s t →* Pair s' t'.
+Proof.
+  intros. eapply star_trans.
+  - apply pair_star_l, H.
+  - apply pair_star_r, H0.
+Qed.
+
+Lemma app_star_l s s' t :
+  s →* s' -> App s t →* App s' t.
+Proof.
+  intros. induction H ; eauto using step, full_step, star.
+Qed.
+
+Lemma app_star_r s t t' :
+  t →* t' -> App s t →* App s t'.
+Proof.
+  intros. induction H ; eauto using step, full_step, star.
+Qed.
+
+Lemma app_star s s' t t' :
+  s →* s' ->  t →* t' -> App s t →* App s' t'.
+Proof.
+  intros. eapply star_trans.
+  apply app_star_l, H.
+  apply app_star_r, H0.
+Qed.
+
+Lemma let_star_l s s' t :
+  s →* s' -> Let s t →* Let s' t.
+Proof.
+  intros. induction H ; eauto using step, full_step, star.
+Qed.
+
+Lemma let_star_r s t t' :
+  t →* t' -> Let s t →* Let s t'.
+Proof.
+  intros. induction H ; eauto using step, full_step, star.
+Qed.
+
+Lemma let_star s s' t t' :
+  s →* s' ->  t →* t' -> Let s t →* Let s' t'.
+Proof.
+  intros. eapply star_trans.
+  apply let_star_l, H.
+  apply let_star_r, H0.
+Qed.
+
+Lemma abs_star s s' :
+  s →* s' -> Abs s →* Abs s'.
+Proof.
+  intros. induction H ; eauto using step, full_step, star.
 Qed.
 
 End TargetCalculus.
