translation.v
@@ -11,39 +11,352 @@ Definition translate_label (l : source_calculus.label) : target_calculus.label.
   rewrite <- label_eq. exact l.
 Defined.
 
-Definition reify_pair (p : term * term) : term := Pair (fst p) (snd p).
-
 Notation "l @ m" := (App (App Join l) m) (at level 70).
 
-Fixpoint translation (e : source_calculus.prefix) : (target_calculus.term * target_calculus.term) :=
+Definition eta_fst (e : target_calculus.term) := match e with
+| Pair e1 _ => e1
+| _ => App Fst e
+end.
+
+Definition eta_snd (e : target_calculus.term) := match e with
+| Pair _ e2 => e2
+| _ => App Snd e
+end.
+
+Fixpoint translation (e : source_calculus.prefix) : target_calculus.term :=
   match e with
-  | source_calculus.Hole => (Const 0, Label bottom)
-  | source_calculus.Const k => (Const k, Label bottom)
-  | source_calculus.Var x => (App Fst (Var x), App Snd (Var x))
-  | source_calculus.Abs e => (Abs (reify_pair (translation e)), Label bottom)
-  | source_calculus.App e1 e2 =>
-     (App Fst (App (fst (translation e1)) (reify_pair (translation e2))),
-     (snd (translation e1)) @ (App Snd (App (fst (translation e1)) (reify_pair (translation e2)))))
-  | source_calculus.Let e1 e2 => (Let (reify_pair (translation e1)) (fst (translation e2)),
-                              Let (reify_pair (translation e1)) (snd (translation e2)))
-  | source_calculus.Label e l => (fst (translation e), snd (translation e))
+  | source_calculus.Hole => Pair (Const 0) (Label bottom)
+  | source_calculus.Const k => Pair (Const k) (Label bottom)
+  | source_calculus.Var x => Var x
+  | source_calculus.Abs e => Pair (Abs (translation e)) (Label bottom)
+  | source_calculus.App e1 e2 => Pair
+     (App Fst (App (eta_fst (translation e1)) (translation e2)))
+     ((eta_snd (translation e1)) @ (App Snd (App (eta_fst (translation e1)) (translation e2))))
+  | source_calculus.Let e1 e2 => Pair
+      (Let (translation e1) (eta_fst (translation e2)))
+      (Let (translation e1) (eta_snd (translation e2)))
+  | source_calculus.Label e l => Pair
+      (eta_fst (translation e))
+      ((Label (translate_label l)) @ (eta_snd (translation e)))
   end.
 
+Inductive eta_eq : term -> term -> Prop :=
+| EtaEqR s : eta_eq s s
+| EtaEqS s t : eta_eq s t -> eta_eq t s
+| EtaEqTrans s t u : eta_eq s t -> eta_eq t u -> eta_eq s u
+| EtaEqEta s : eta_eq (Pair (App Fst s) (App Snd s)) s
+| EtaEqFst s t : eta_eq (App Fst (Pair s t)) s
+| EtaEqSnd s t : eta_eq (App Snd (Pair s t)) t
+| EtaEqAbs s t : eta_eq s t -> eta_eq (Abs s) (Abs t)
+| EtaEqApp s s' t t' : eta_eq s s' -> eta_eq t t' -> eta_eq (App s t) (App s' t')
+| EtaEqLet s s' t t' : eta_eq s s' -> eta_eq t t' -> eta_eq (Let s t) (Let s' t')
+| EtaEqPair s s' t t' : eta_eq s s' -> eta_eq t t' -> eta_eq (Pair s t) (Pair s' t').
+
 Notation "⦇ e ⦈" := (translation e).
-Notation "*⦇ e ⦈*" := (reify_pair (translation e)).
 
-Notation "s → t" := (source_calculus.step s t) (at level 70).
-Notation "s →@* t" := (target_calculus.star_ext s t) (at level 70).
+Notation "s → t" := (source_calculus.full_step s t) (at level 70).
+Notation "s →* t" := (target_calculus.star s t) (at level 70).
 
-Lemma simulation (e f : source_calculus.prefix) (He : is_term e) (Hf : is_term f) :
-  e → f  -> *⦇e⦈* →@* *⦇f⦈*.
+Instance Ids_prefix : Ids prefix. derive. Defined.
+Instance Rename_prefix : Rename prefix. derive. Defined.
+Instance Subst_prefix : Subst prefix. derive. Defined.
+Instance SubstLemmas_prefix : SubstLemmas prefix. derive. Defined.
+
+Instance Ids_term : Ids term. derive. Defined.
+Instance Rename_term : Rename term. derive. Defined.
+Instance Subst_term : Subst term. derive. Defined.
+Instance SubstLemmas_term : SubstLemmas term. derive. Defined.
+
+Lemma fst_ren s xi :
+  ⦇s⦈.[ren xi] = ⦇s.[ren xi]⦈ -> (eta_fst ⦇s⦈).[ren xi] = eta_fst ⦇s.[ren xi]⦈.
+Proof.
+  revert xi. destruct s ; intros xi H ; try autosubst ; simpl ; inversion H ; f_equal.
+Qed.
+
+Lemma snd_ren s xi :
+  ⦇s⦈.[ren xi] = ⦇s.[ren xi]⦈ -> (eta_snd ⦇s⦈).[ren xi] = eta_snd ⦇s.[ren xi]⦈.
+Proof.
+  revert xi. destruct s ; intros xi H ; try autosubst ; simpl ; inversion H ; f_equal.
+Qed.
+
+Lemma ren_translation xi : translation >>> (subst (xi >>> ids)) = subst (xi >>> ids) >>> translation.
+Proof.
+  f_ext. intros s. simpl. revert xi. induction s ; intros ; asimpl ; autosubst_unfold ; try now autorew ;
+  repeat f_equal ; eauto using fst_ren, snd_ren.
+Qed.
+
+Hint Rewrite @ren_translation : autosubst.
+
+Lemma ren_up sigma :
+    up sigma >>> translation = up (sigma >>> translation).
+Proof. autosubst. Qed.
+
+Lemma five_one e sigma (H1 : is_term e) :
+   ⦇e⦈.[sigma >>> translation] →* ⦇e.[sigma]⦈ /\ (eta_fst ⦇e⦈).[sigma >>> translation] →* eta_fst ⦇e.[sigma]⦈ /\ (eta_snd ⦇e⦈).[sigma >>> translation] →* eta_snd ⦇e.[sigma]⦈.
+Proof.
+  revert sigma. induction e ; intros ; simpl ; eauto using step, star ; inversion H1 ; subst ; repeat split.
+  - constructor.
+  - destruct (sigma x) ; eauto using star, full_step, step.
+  - destruct (sigma x) ; eauto using star, full_step, step.
+  - apply pair_star_l. rewrite <- ren_up. apply abs_star. now apply IHe.
+  - rewrite <- ren_up. apply abs_star. now apply IHe.
+  - constructor.
+  - apply pair_star.
+    + apply app_star_r. apply app_star.
+       * now apply IHe1.
+       * now apply IHe2.
+    + apply app_star.
+       * apply app_star_r. now apply IHe1.
+       * apply app_star_r. apply app_star.
+          { now apply IHe1. }
+          { now apply IHe2. }
+  - apply app_star_r. apply app_star.
+     + now apply IHe1.
+     + now apply IHe2.
+  - apply app_star.
+     + apply app_star_r. now apply IHe1.
+     + apply app_star_r. apply app_star.
+        * now apply IHe1.
+        * now apply IHe2.
+  - apply pair_star.
+    + apply let_star.
+       * now apply IHe.
+       * rewrite <- ren_up. now apply IHe0.
+    + apply let_star.
+       * now apply IHe.
+       * rewrite <- ren_up. now apply IHe0.
+  - apply let_star.
+    + now apply IHe.
+    + rewrite <- ren_up. now apply IHe0.
+  - apply let_star.
+    + now apply IHe.
+    + rewrite <- ren_up. now apply IHe0.
+  - apply pair_star.
+    + now apply IHe.
+    + apply app_star_r. now apply IHe.
+  - now apply IHe.
+  - apply app_star_r. now apply IHe.
+Qed.
+
+Lemma five_one' e1 e2 (H1 : is_term e1) (H2 : is_term e2) :
+  ⦇e1⦈.[⦇e2⦈/] →* ⦇e1.[e2/]⦈ /\ (eta_fst ⦇e1⦈).[⦇e2⦈/] →* eta_fst ⦇e1.[e2/]⦈ /\ (eta_snd ⦇e1⦈).[⦇e2⦈/] →* eta_snd ⦇e1.[e2/]⦈.
+Proof.
+  repeat split.
+  - assert (exists sigma, ⦇e1⦈.[scons (translation e2) ids] = ⦇e1⦈.[sigma >>> translation] /\ ⦇e1.[scons e2 ids]⦈ = ⦇e1.[sigma]⦈).
+    { unfold ids. unfold Ids_term. unfold funcomp. unfold scons.
+      exists (fun x => match x with 0 => e2 | S y => source_calculus.Var y end).
+      split ; auto. repeat f_equal ; f_ext ; intros ; destruct x ; auto.
+    }
+    destruct H as [sigma [HL HR]]. autorew. now apply five_one.
+  - assert (exists sigma, (eta_fst ⦇e1⦈).[scons (translation e2) ids] = (eta_fst ⦇e1⦈).[sigma >>> translation] /\ eta_fst ⦇e1.[scons e2 ids]⦈ = eta_fst ⦇e1.[sigma]⦈).
+    { unfold ids. unfold Ids_term. unfold funcomp. unfold scons.
+      exists (fun x => match x with 0 => e2 | S y => source_calculus.Var y end).
+      split ; auto. repeat f_equal ; f_ext ; intros ; destruct x ; auto.
+    }
+    destruct H as [sigma [HL HR]]. autorew. now apply five_one.
+  - assert (exists sigma, (eta_snd ⦇e1⦈).[scons (translation e2) ids] = (eta_snd ⦇e1⦈).[sigma >>> translation] /\ eta_snd ⦇e1.[scons e2 ids]⦈ = eta_snd ⦇e1.[sigma]⦈).
+    { unfold ids. unfold Ids_term. unfold funcomp. unfold scons.
+      exists (fun x => match x with 0 => e2 | S y => source_calculus.Var y end).
+      split ; auto. repeat f_equal ; f_ext ; intros ; destruct x ; auto.
+    }
+    destruct H as [sigma [HL HR]]. autorew. now apply five_one.
+Qed.
+
+Lemma eta_pair x :
+  eta_eq (Pair (eta_fst x) (eta_snd x)) x.
+Proof.
+  induction x ; simpl ; eauto using eta_eq.
+Qed.
+
+Lemma simulation_beta s t (H : is_term (source_calculus.App (source_calculus.Abs s) t)) :
+  exists u, ⦇source_calculus.App (source_calculus.Abs s) t⦈ →* u /\ eta_eq u ⦇s.[t/]⦈.
+Proof.
+  ainv. simpl. esplit. split.
+  - eapply star_trans.
+    + apply pair_star.
+      * apply app_star_r. apply star_step, FullStep_step, Step_beta.
+      * apply star_step, FullStep_step, Step_neutral.
+    + eapply star_trans.
+       * apply pair_star.
+         { apply app_star_r. now apply five_one'. }
+         { apply app_star_r. apply star_step, FullStep_step, Step_beta. }
+       * apply pair_star_r. apply app_star_r. now apply five_one'.
+  - apply EtaEqEta.
+Qed.
+
+Lemma simulation_let s t (H : is_term (source_calculus.Let s t)) :
+  exists u, ( ⦇source_calculus.Let s t⦈ →* u /\ eta_eq u ⦇t.[s/]⦈).
+Proof.
+  ainv. simpl. esplit. split.
+  - eapply star_trans.
+    + apply pair_star ; apply star_step, FullStep_step, Step_let.
+    + apply pair_star ; now apply five_one'.
+  - apply eta_pair.
+Qed.
+
+Lemma simulation_label s l t (H : is_term (source_calculus.App (source_calculus.Label s l) t)) :
+  exists u, ⦇source_calculus.App (source_calculus.Label s l ) t⦈ →* u  /\ eta_eq u ⦇source_calculus.Label (source_calculus.App s t) l⦈.
+Proof.
+  ainv. simpl. repeat esplit.
+  - apply pair_star_r, star_step, FullStep_step, Step_assoc.
+  - constructor.
+Qed.
+
+Lemma simulation_step (e f : source_calculus.prefix) (He : is_term e) (Hf : is_term f) :
+  source_calculus.step e f  -> exists u, ⦇e⦈ →* u /\ eta_eq u ⦇f⦈.
+Proof.
+  intros. destruct H.
+  - now apply simulation_beta.
+  - now apply simulation_let.
+  - now apply simulation_label.
+Qed.
+
+Lemma eta_fst_app s :
+  App Fst s →* eta_fst s.
+Proof.
+  destruct s ; simpl ; try constructor. apply star_step, FullStep_step, Step_fst.
+Qed.
+
+Lemma eta_snd_app s :
+  App Snd s →* eta_snd s.
+Proof.
+  destruct s ; simpl ; try constructor. apply star_step, FullStep_step, Step_snd.
+Qed.
+
+Lemma eta_fst_step s u :
+  target_calculus.full_step s u -> eta_fst s →* eta_fst u.
+Proof.
+  intros. destruct H ; simpl.
+  - destruct H ; simpl.
+    + eapply star_trans.
+       * apply app_star_r. apply star_step, FullStep_step, Step_beta.
+       * apply eta_fst_app.
+    + eapply star_trans.
+       * apply app_star_r. apply star_step, FullStep_step, Step_let.
+       * apply eta_fst_app.
+    + eapply star_trans.
+       * apply app_star_r. apply star_step, FullStep_step, Step_fst.
+       * apply eta_fst_app.
+    + eapply star_trans.
+       * apply app_star_r. apply star_step, FullStep_step, Step_snd.
+       * apply eta_fst_app.
+    + apply app_star_r. apply star_step, FullStep_step, Step_join.
+    + apply app_star_r. apply star_step, FullStep_step, Step_assoc.
+    + eapply star_trans.
+       * apply app_star_r. apply star_step, FullStep_step, Step_neutral.
+       * apply eta_fst_app.
+  - apply app_star_r. apply abs_star. econstructor ; eauto. constructor.
+  - apply app_star_r. apply app_star_l. econstructor ; eauto. constructor.
+  - apply app_star_r. apply app_star_r. econstructor ; eauto. constructor.
+  - apply app_star_r. apply let_star_l. econstructor ; eauto. constructor.
+  - apply app_star_r. apply let_star_r. econstructor ; eauto. constructor.
+  - econstructor ; eauto. constructor.
+  - constructor.
+Qed.
+
+Lemma eta_snd_step s u :
+  target_calculus.full_step s u -> eta_snd s →* eta_snd u.
+Proof.
+  intros. destruct H ; simpl.
+  - destruct H ; simpl.
+    + eapply star_trans.
+       * apply app_star_r. apply star_step, FullStep_step, Step_beta.
+       * apply eta_snd_app.
+    + eapply star_trans.
+       * apply app_star_r. apply star_step, FullStep_step, Step_let.
+       * apply eta_snd_app.
+    + eapply star_trans.
+       * apply app_star_r. apply star_step, FullStep_step, Step_fst.
+       * apply eta_snd_app.
+    + eapply star_trans.
+       * apply app_star_r. apply star_step, FullStep_step, Step_snd.
+       * apply eta_snd_app.
+    + apply app_star_r. apply star_step, FullStep_step, Step_join.
+    + apply app_star_r. apply star_step, FullStep_step, Step_assoc.
+    + eapply star_trans.
+       * apply app_star_r. apply star_step, FullStep_step, Step_neutral.
+       * apply eta_snd_app.
+  - apply app_star_r. apply abs_star. econstructor ; eauto. constructor.
+  - apply app_star_r. apply app_star_l. econstructor ; eauto. constructor.
+  - apply app_star_r. apply app_star_r. econstructor ; eauto. constructor.
+  - apply app_star_r. apply let_star_l. econstructor ; eauto. constructor.
+  - apply app_star_r. apply let_star_r. econstructor ; eauto. constructor.
+  - constructor.
+  - econstructor ; eauto. constructor.
+Qed.
+
+Lemma eta_fst_star s u :
+  s →* u -> eta_fst s →* eta_fst u.
 Proof.
   intros. induction H.
-  - admit.
-  - admit.
-  - eauto using star_ext.
-  - admit.
-  - admit.
-Admitted.
+  - constructor.
+  - apply eta_fst_step in H. eapply star_trans ; eauto.
+Qed.
+
+Lemma eta_snd_star s u :
+  s →* u -> eta_snd s →* eta_snd u.
+Proof.
+  intros. induction H.
+  - constructor.
+  - apply eta_snd_step in H. eapply star_trans ; eauto.
+Qed.
+
+Lemma eq_app_fst_eta_fst s :
+  eta_eq (App Fst s) (eta_fst s).
+Proof.
+  destruct s ; eauto using eta_eq.
+Qed.
+
+Lemma eq_app_snd_eta_snd s :
+  eta_eq (App Snd s) (eta_snd s).
+Proof.
+  destruct s ; eauto using eta_eq.
+Qed.
+
+Lemma eta_eq_fst s t :
+  eta_eq s t -> eta_eq (eta_fst s) (eta_fst t).
+Proof.
+  induction 1 ; eauto using eta_eq, eq_app_fst_eta_fst.
+Qed.
+
+Lemma eta_eq_snd s t :
+  eta_eq s t -> eta_eq (eta_snd s) (eta_snd t).
+Proof.
+  induction 1 ; eauto using eta_eq, eq_app_snd_eta_snd.
+Qed.
+
+Lemma simulation (e f : source_calculus.prefix) (He : is_term e) (Hf : is_term f) :
+  e → f  -> exists u, ⦇e⦈  →* u /\ eta_eq u ⦇f⦈.
+Proof.
+  intros. induction H ; ainv ; simpl.
+  - now apply simulation_step.
+  - destruct IHfull_step as [x []]; auto. repeat esplit.
+    + apply pair_star_l, abs_star. eassumption.
+    + eauto using eta_eq.
+  - destruct IHfull_step as [x []]; auto. repeat esplit.
+    + apply pair_star.
+       * apply app_star_r, app_star_l. apply eta_fst_star. eassumption.
+       * apply app_star.
+          { apply app_star_r. apply eta_snd_star. eassumption. }
+          { apply app_star_r, app_star_l. apply eta_fst_star. eassumption. }
+    + apply EtaEqPair ; eauto 7 using eta_eq, eta_eq_fst, eta_eq_snd.
+  - destruct IHfull_step as [x []]; auto. repeat esplit. apply pair_star.
+    + apply app_star_r, app_star_r. eassumption.
+    + apply app_star_r, app_star_r, app_star_r. eassumption.
+    + apply EtaEqPair ; eauto using eta_eq.
+  - destruct IHfull_step as [x []] ; auto. repeat esplit.
+    + apply pair_star ; apply let_star_l ; eassumption.
+    + apply EtaEqPair ; eauto using eta_eq.
+  - destruct IHfull_step as [x []] ; auto. repeat esplit.
+    + apply pair_star.
+       * apply let_star_r. apply eta_fst_star. eassumption.
+       * apply let_star_r. apply eta_snd_star. eassumption.
+    + apply EtaEqPair ; eauto using eta_eq, eta_eq_fst, eta_eq_snd.
+  - destruct IHfull_step as [x []] ; auto. repeat esplit.
+    + apply pair_star.
+       * apply eta_fst_star. eassumption.
+       * apply app_star_r. apply eta_snd_star. eassumption.
+    + apply EtaEqPair ; eauto using eta_eq, eta_eq_fst, eta_eq_snd.
+Qed.
 
 End Translation.
